Define composition of var_substs

Terms/Perm.v
@@ -4,11 +4,11 @@ Require Import Top.Terms.Term.
 Require Import Top.FinSet.FinMod.
 Require Import Top.FinSet.FinModComp.
 
-(** A var_subst is like a substitution, but induced by a map [V ->
+(** A [var_subst] is like a substitution, but induced by a map [V ->
     V]. Composing on the left with [varTerm] gives the substitution
     itself. *)
 
-Section Perm.
+Section var_subst.
   Variable V : Type.
   Variable F : Type.
   Variable a : F -> nat.
@@ -31,4 +31,23 @@ Section Perm.
     apply (compose_fin_mod decV decV (decTerm V F a decV decF));
       first [ apply finH | apply fin_mod_i | contradiction ].
   Qed.
-End Perm.
+
+  Definition compose_var_subst : var_subst -> var_subst -> var_subst :=
+    fun t s =>
+      match t, s with
+        exist _ g gH, exist _ f fH =>
+        exist _ (compose g f) (compose_fin_endo decV fH gH)
+      end.
+
+  Lemma proj1_sig_compose_var_subst t s
+    : proj1_sig (compose_var_subst t s) = compose (proj1_sig t) (proj1_sig s).
+  Proof.
+    destruct t as [ g gH ]; destruct s as [ f fH ]; auto.
+  Qed.
+End var_subst.
+
+Arguments var_subst V.
+Arguments var_subst_subst {V F} a s v.
+Arguments fin_subst_var_subst {V F} a decV decF.
+Arguments compose_var_subst {V} decV t s.
+Arguments proj1_sig_compose_var_subst {V} decV t s.
